theories/bunch_decomp.v
@@ -1,0 +1,183 @@
+(** Inductive representation for decomposition of bunches, and associated properties *)
+From Coq Require Import ssreflect.
+From stdpp Require Import prelude gmap functions.
+From Equations Require Import Equations.
+From bunched Require Export syntax terms.
+
+(** * Alternative representation of decomposition of bunches *)
+(** We have an inductive type that characterizes when a bunch can be
+  decomposed into a context and a sub-bunch. This essentially gives an
+  us an inductive reasoning principle for equations [fill Π Δ = Δ']. *)
+Inductive bunch_decomp :
+  bunch → bunch_ctx → bunch → Prop :=
+| decomp_id Δ : bunch_decomp Δ [] Δ
+| decomp_comma_1 Δ1 Δ2 Π Δ :
+    bunch_decomp Δ1 Π Δ →
+    bunch_decomp (Δ1,,Δ2)%B (Π ++ [CtxCommaL Δ2]) Δ
+| decomp_comma_2 Δ1 Δ2 Π Δ :
+    bunch_decomp Δ2 Π Δ →
+    bunch_decomp (Δ1,,Δ2)%B (Π ++ [CtxCommaR Δ1]) Δ
+| decomp_semic_1 Δ1 Δ2 Π Δ :
+    bunch_decomp Δ1 Π Δ →
+    bunch_decomp (Δ1;,Δ2)%B (Π ++ [CtxSemicL Δ2]) Δ
+| decomp_semic_2 Δ1 Δ2 Π Δ :
+    bunch_decomp Δ2 Π Δ →
+    bunch_decomp (Δ1;,Δ2)%B (Π ++ [CtxSemicR Δ1]) Δ.
+
+(** [bunch_decomp Δ' Π Δ] completely characterizes [fill Π Δ = Δ'] *)
+Lemma bunch_decomp_correct Δ Π Δ' :
+  bunch_decomp Δ Π Δ' → Δ = fill Π Δ'.
+Proof. induction 1; rewrite ?fill_app /= //; try by f_equiv. Qed.
+
+Lemma bunch_decomp_complete' Π Δ' :
+  bunch_decomp (fill Π Δ') Π Δ'.
+Proof.
+  revert Δ'. remember (reverse Π) as Πr.
+  revert Π HeqΠr.
+  induction Πr as [|HΠ Πr]=>Π HeqΠr.
+  { assert (Π = []) as ->.
+    {  by eapply (inj reverse). }
+    simpl. intros. econstructor. }
+  intros Δ'.
+  assert (Π = reverse Πr ++ [HΠ]) as ->.
+  { by rewrite -reverse_cons HeqΠr reverse_involutive. }
+  rewrite fill_app /=.
+  revert Δ'.
+  induction HΠ=>Δ' /=; econstructor; eapply IHΠr; by rewrite reverse_involutive.
+Qed.
+
+Lemma bunch_decomp_complete Δ Π Δ' :
+  (fill Π Δ' = Δ) →
+  bunch_decomp Δ Π Δ'.
+Proof. intros <-. apply bunch_decomp_complete'. Qed.
+
+Lemma fill_is_frml Π Δ ϕ :
+  fill Π Δ = frml ϕ →
+  Π = [] ∧ Δ = frml ϕ.
+Proof.
+  revert Δ. induction Π as [| F C IH]=>Δ; first by eauto.
+  destruct F ; simpl ; intros H1 ;
+    destruct (IH _ H1) as [HC HΔ] ; by simplify_eq/=.
+Qed.
+
+Lemma bunch_decomp_app C C0 Δ Δ0 :
+  bunch_decomp Δ C0 Δ0 →
+  bunch_decomp (fill C Δ) (C0 ++ C) Δ0.
+Proof.
+  revert Δ Δ0 C0.
+  induction C as [|F C]=>Δ Δ0 C0.
+  { simpl. by rewrite app_nil_r. }
+  intros HD.
+  replace (C0 ++ F :: C) with ((C0 ++ [F]) ++ C); last first.
+  { by rewrite -assoc. }
+  apply IHC. destruct F; simpl; by econstructor.
+Qed.
+
+Lemma bunch_decomp_ctx C C' Δ ϕ :
+  bunch_decomp (fill C Δ) C' (frml ϕ) →
+  ((∃ C0, bunch_decomp Δ C0 (frml ϕ) ∧ C' = C0 ++ C) ∨
+   (∃ (C0 C1 : bunch → bunch_ctx),
+       (∀ Δ Δ', fill (C0 Δ) Δ' = fill (C1 Δ') Δ) ∧
+       (∀ Δ', fill (C1 Δ') Δ = fill C' Δ') ∧
+       (∀ A, bunch_decomp (fill C A) (C0 A) (frml ϕ)))).
+Proof.
+  revert Δ C'.
+  induction C as [|F C]=>Δ C'; simpl.
+  { remember (frml ϕ) as Γ1. intros Hdec.
+    left. eexists. rewrite right_id. split; done. }
+  simpl. intros Hdec.
+  destruct (IHC _ _ Hdec) as [IH|IH].
+  - destruct IH as [C0 [HC0 HC]].
+    destruct F; simpl in *.
+    + inversion HC0; simplify_eq/=.
+      * left. eexists; split; eauto.
+        rewrite -assoc //.
+      * right.
+        exists (λ A, (Π ++ [CtxCommaR A]) ++ C).
+        exists (λ A, ([CtxCommaL (fill Π A)] ++ C)).
+        repeat split.
+        { intros A B. by rewrite /= -!assoc /= !fill_app. }
+        { intros A. by rewrite /= -!assoc /= !fill_app. }
+        { intros A. apply bunch_decomp_app. by econstructor. }
+    + inversion HC0; simplify_eq/=.
+      * right.
+        exists (λ A, (Π ++ [CtxCommaL A]) ++ C).
+        exists (λ A, ([CtxCommaR (fill Π A)] ++ C)).
+        repeat split.
+        { intros A B. by rewrite /= -!assoc /= !fill_app. }
+        { intros A. by rewrite /= -!assoc /= !fill_app. }
+        { intros A. apply bunch_decomp_app. by econstructor. }
+      * left. eexists; split; eauto.
+        rewrite -assoc //.
+    + inversion HC0; simplify_eq/=.
+      * left. eexists; split; eauto.
+        rewrite -assoc //.
+      * right.
+        exists (λ A, (Π ++ [CtxSemicR A]) ++ C).
+        exists (λ A, ([CtxSemicL (fill Π A)] ++ C)).
+        repeat split.
+        { intros A B. by rewrite /= -!assoc /= !fill_app. }
+        { intros A. by rewrite /= -!assoc /= !fill_app. }
+        { intros A. apply bunch_decomp_app. by econstructor. }
+    + inversion HC0; simplify_eq/=.
+      * right.
+        exists (λ A, (Π ++ [CtxSemicL A]) ++ C).
+        exists (λ A, ([CtxSemicR (fill Π A)] ++ C)).
+        repeat split.
+        { intros A B. by rewrite /= -!assoc /= !fill_app. }
+        { intros A. by rewrite /= -!assoc /= !fill_app. }
+        { intros A. apply bunch_decomp_app. by econstructor. }
+      * left. eexists; split; eauto.
+        rewrite -assoc //.
+  - right.
+    destruct IH as (C0 & C1 & HC0 & HC1 & HC).
+    exists (λ A, C0 (fill_item F A)), (λ A, F::C1 A). repeat split.
+    { intros A B. simpl. rewrite -HC0 //. }
+    { intros B. rewrite -HC1 //. }
+    intros A. apply HC.
+Qed.
+
+
+(* facts about terms *)
+Lemma bterm_ctx_act_decomp `{!EqDecision V, !Countable V} (T : bterm V)
+  (Δs : V → bunch) ϕ Π :
+  linear_bterm T →
+  bterm_ctx_act T Δs = fill Π (frml ϕ) →
+  ∃ (j : V) Π₀ , j ∈ term_fv T ∧ Δs j = fill Π₀ (frml ϕ) ∧
+   (∀ Δ, bterm_ctx_act T (<[j:=(fill Π₀ Δ)]>Δs) = fill Π Δ).
+Proof.
+  revert Π. induction T=>Π Hlin.
+  - simpl.
+    intros Hx. exists x, Π. repeat split; auto.
+    { simp term_fv. set_solver. }
+    intros Γ. by rewrite fn_lookup_insert.
+  - simpl. simp linear_bterm in Hlin.
+    destruct Hlin as (Ht12 & Hlin1 & Hlin2).
+    intros Ht. symmetry in Ht.
+    apply bunch_decomp_complete in Ht.
+    inversion Ht; simplify_eq/=.
+    + apply bunch_decomp_correct in H3.
+      specialize (IHT1 _ Hlin1 H3) as (j & Π₀ & Hjfv & Hj & HH).
+      exists j, Π₀. repeat split; auto.
+      { simp term_fv. set_solver. }
+      intros Γ. rewrite fill_app/=. f_equiv.
+      * apply HH.
+      * assert (j ∉ term_fv T2).
+        { set_solver. }
+        apply bterm_ctx_act_fv.
+        intros i. destruct (decide (i = j)) as [->|?].
+        { naive_solver. }
+        rewrite fn_lookup_insert_ne//.
+    + apply bunch_decomp_correct in H3.
+      specialize (IHT2 _ Hlin2 H3) as (j & Π₀ & Hjfv & Hj & HH).
+      exists j, Π₀. repeat split; auto.
+      { simp term_fv. set_solver. }
+      intros Γ. rewrite fill_app/=. f_equiv.
+      * assert (j ∉ term_fv T1).
+        { set_solver. }
+        apply bterm_ctx_act_fv.
+        intros i. destruct (decide (i = j)) as [->|?].
+        { naive_solver. }
+        rewrite fn_lookup_insert_ne//.
+      * apply HH.
+Qed.
