README.md
@@ -1,2 +1,20 @@
-Formalization of the BI sequent calculus and an algebraic/semantic proof of cut elimination.
-WIP
+A semantic cut admissibility proof for the logic of Bunched Implications and extensions.
+
+We formalize the sequent calculus of BI and give an algebraic proof of
+cut admissibility. We parametrize the calculus by an arbitrary
+collection of "simple structural rules" (see `theories/seqcalc.v` for
+the definition).
+
+Structure:
+- `syntax.v`, `terms.v` -- formulas of BI and "bunched terms".
+  A bunched term is essential a formula built up only from `∗/,` and
+  `∧/;` and variables.
+- `interp.v` -- interpretation of formulas and bunched terms in a BI algebra
+- `seqcalc.v` -- sequent calculus + soundness
+- `bunch_decomp.v` -- helpful lemmas about decompositions of bunches
+- `seqcalc_height.v` -- the same sequent calculus, but with the notion of proof height.
+  Includes proofs of invertibility of some of the rules.
+- `cutelim.v` -- the universal model for cut elimination
+
+We can adapt the same method to modal BI, by "freely" adding an S4-like box modality.
+See `seqcalc_s4.v`, `cutelim_s4.v` etc.
